BananasProgram.thy
@@ -17,23 +17,27 @@ fun binders :: "decl list \<Rightarrow> name set" where
 
 datatype prog = Prog "decl list" expr val
 
-fun typecheck\<^sub>c :: "(name \<times> type list) list \<Rightarrow> (name \<rightharpoonup> type) \<times> name set \<times> funct" where
-  "typecheck\<^sub>c [] = (Map.empty, {}, K \<zero>)" 
-| "typecheck\<^sub>c ((x, ts) # cts) = (
-    let (es, vs, Fs) = typecheck\<^sub>c cts
-    in (es(x \<mapsto> foldr (op \<otimes>) ts \<one>), insert x vs, Fs \<Oplus> (foldr (\<lambda>t f. K t \<Otimes> f) ts (K \<one>))))"
+fun typecheck\<^sub>c\<^sub>e :: "funct \<Rightarrow> (name \<times> type list) list \<Rightarrow> (name \<rightharpoonup> type \<times> type)" where
+  "typecheck\<^sub>c\<^sub>e F [] y = None" 
+| "typecheck\<^sub>c\<^sub>e F ((x, ts) # cts) y = 
+    (if y = x then Some (foldr (op \<otimes>) ts \<one>, \<mu> F) else typecheck\<^sub>c\<^sub>e F cts y)"
 
-fun bind_with_name :: "name \<Rightarrow> (name \<rightharpoonup> type) \<times> name set \<times> funct \<Rightarrow> static_environment" where
-  "bind_with_name n (es, vs, Fs) = \<lparr> 
-      var\<^sub>e_type = map_option (\<lambda>t. (t, Named n)) o es, 
-      var\<^sub>v_type = \<lambda>x. if x \<in> vs then Some (Named n) else None, 
-      var\<^sub>t_type = [n \<mapsto> Fs] \<rparr>"
+definition typecheck\<^sub>c\<^sub>v :: "funct \<Rightarrow> (name \<times> type list) list \<Rightarrow> (name \<rightharpoonup> type)" where
+  "typecheck\<^sub>c\<^sub>v F cts x = (if x \<in> fst ` set cts then Some (\<mu> F) else None)"
+
+definition typecheck\<^sub>c\<^sub>t :: "(name \<times> type list) list \<Rightarrow> funct" where
+  "typecheck\<^sub>c\<^sub>t cts = foldr (\<lambda>(x, ts). op \<Oplus> (foldr (op \<Otimes> o K) ts (K \<one>))) cts (K \<zero>)"
+
+definition typecheck\<^sub>d :: "name \<Rightarrow> (name \<times> type list) list \<Rightarrow> static_environment" where
+  "typecheck\<^sub>d n cts = (
+      let F = typecheck\<^sub>c\<^sub>t cts 
+      in \<lparr> var\<^sub>e_type = typecheck\<^sub>c\<^sub>e F cts, var\<^sub>v_type = typecheck\<^sub>c\<^sub>v F cts, var\<^sub>t_type = [n \<mapsto> F] \<rparr>)"
 
 inductive typecheck_decl :: "static_environment \<Rightarrow> decl \<Rightarrow> static_environment \<Rightarrow> bool" 
     (infix "\<Turnstile> _ :" 60) where
-  tcd_type [simp]: "\<Gamma> \<Turnstile> TypeDecl x cts : combine \<Gamma> (bind_with_name x (typecheck\<^sub>c cts))"
-| tcd_val [simp]: "\<Gamma> \<turnstile> v : t \<Longrightarrow> \<Gamma> \<Turnstile> ValDecl x v : extend\<^sub>v x t \<Gamma>"
-| tcd_expr [simp]: "\<Gamma> \<turnstile> e : t\<^sub>1 \<rightarrow> t\<^sub>2 \<Longrightarrow> \<Gamma> \<Turnstile> ExprDecl x e : extend\<^sub>e x (t\<^sub>1, t\<^sub>2) \<Gamma>"
+  tcd_type [simp]: "\<Gamma> \<Turnstile> TypeDecl x cts : combine\<^sub>s \<Gamma> (typecheck\<^sub>d x cts)"
+| tcd_val [simp]: "\<Gamma> \<turnstile> v : t \<Longrightarrow> \<Gamma> \<Turnstile> ValDecl x v : extend\<^sub>v\<^sub>s x t \<Gamma>"
+| tcd_expr [simp]: "\<Gamma> \<turnstile> e : t\<^sub>1 \<rightarrow> t\<^sub>2 \<Longrightarrow> \<Gamma> \<Turnstile> ExprDecl x e : extend\<^sub>e\<^sub>s x (t\<^sub>1, t\<^sub>2) \<Gamma>"
 
 inductive_cases [elim]: "\<Gamma> \<Turnstile> TypeDecl x F : \<Gamma>'"
 inductive_cases [elim]: "\<Gamma> \<Turnstile> ValDecl x v : \<Gamma>'"
@@ -42,173 +46,164 @@ inductive_cases [elim]: "\<Gamma> \<Turnstile> ExprDecl x e : \<Gamma>'"
 inductive typecheck_decls :: "static_environment \<Rightarrow> decl list \<Rightarrow> static_environment \<Rightarrow> bool" 
     (infix "\<Turnstile> _ ::" 60) where
   tcd_nil [simp]: "\<Gamma> \<Turnstile> [] :: \<Gamma>"
-| tcd_cons [simp]: "\<Gamma> \<Turnstile> \<delta> : \<Gamma>' \<Longrightarrow> binders\<^sub>d \<delta> \<inter> binders \<Lambda> = {} \<Longrightarrow> \<Gamma>' \<Turnstile> \<Lambda> :: \<Gamma>'' \<Longrightarrow> 
+| tcd_cons [simp]: "\<Gamma> \<Turnstile> \<delta> : \<Gamma>' \<Longrightarrow> binders\<^sub>d \<delta> \<inter> domain\<^sub>s \<Gamma> = {} \<Longrightarrow> \<Gamma>' \<Turnstile> \<Lambda> :: \<Gamma>'' \<Longrightarrow> 
     \<Gamma> \<Turnstile> \<delta> # \<Lambda> :: \<Gamma>''"
 
 inductive_cases [elim]: "\<Gamma> \<Turnstile> [] :: \<Gamma>'"
 inductive_cases [elim]: "\<Gamma> \<Turnstile> \<delta> # \<Lambda> :: \<Gamma>'"
 
-inductive typecheck_prog :: "prog \<Rightarrow> (name \<rightharpoonup> type \<times> type) \<Rightarrow> (name \<rightharpoonup> funct) \<Rightarrow> type \<Rightarrow> bool" 
-    (infix "\<TTurnstile> _ & _ :" 60) where
-  tcp_prog [simp]: "Map.empty & Map.empty \<Turnstile> \<Lambda> :: \<Gamma> & \<Sigma> \<Longrightarrow> \<Gamma> & \<Sigma> \<turnstile> e : t\<^sub>1 \<rightarrow> t\<^sub>2 \<Longrightarrow> 
-    \<Gamma> & \<Sigma> \<turnstile> v : t\<^sub>1 \<Longrightarrow> Prog \<Lambda> e v \<TTurnstile> \<Gamma> & \<Sigma> : t\<^sub>2"
+definition empty_static :: static_environment where
+  "empty_static = \<lparr> var\<^sub>e_type = Map.empty, var\<^sub>v_type = Map.empty, var\<^sub>t_type = Map.empty \<rparr>"
 
-inductive_cases [elim]: "Prog \<Lambda> e v \<TTurnstile> \<Gamma> & \<Sigma> : t"
+inductive typecheck_prog :: "prog \<Rightarrow> static_environment \<Rightarrow> type \<Rightarrow> bool" (infix "\<TTurnstile> _ \<rightarrow> " 60) where
+  tcp_prog [simp]: "empty_static \<Turnstile> \<Lambda> :: \<Gamma> \<Longrightarrow> \<Gamma> \<turnstile> e : t\<^sub>1 \<rightarrow> t\<^sub>2 \<Longrightarrow> \<Gamma> \<turnstile> v : t\<^sub>1 \<Longrightarrow> 
+    Prog \<Lambda> e v \<TTurnstile> \<Gamma> \<rightarrow> t\<^sub>2"
 
-fun assemble_context\<^sub>c :: "name \<Rightarrow> (name \<times> type list) list \<Rightarrow> name \<rightharpoonup> expr" where
-  "assemble_context\<^sub>c n [] = Map.empty"
-| "assemble_context\<^sub>c n ((x, t) # cts) = 
-    (map_option (op \<cdot> \<iota>\<^sub>r) o assemble_context\<^sub>c n cts)(x \<mapsto> \<prec>\<^bsub>n\<^esub> \<cdot> \<iota>\<^sub>l)"
+inductive_cases [elim]: "Prog \<Lambda> e v \<TTurnstile> \<Gamma>  \<rightarrow> t"
 
-primrec assemble_context' :: "decl \<Rightarrow> name \<rightharpoonup> expr" where
-  "assemble_context' (TypeDecl x cts) = assemble_context\<^sub>c x cts"
-| "assemble_context' (ExprDecl x e) = [x \<mapsto> e]"
+definition empty_dynamic :: dynamic_environment where
+  "empty_dynamic = \<lparr> var\<^sub>e_bind = Map.empty, var\<^sub>v_bind = Map.empty, var\<^sub>t_bind = Map.empty \<rparr>"
 
-primrec assemble_context :: "decl list \<Rightarrow> name \<rightharpoonup> expr" where
-  "assemble_context [] = Map.empty"
-| "assemble_context (\<delta> # \<Lambda>) = assemble_context' \<delta> ++ assemble_context \<Lambda>"
+primrec right_inject :: "nat \<Rightarrow> expr" where
+  "right_inject 0 = \<iota>\<^sub>l"
+| "right_inject (Suc x) = \<iota>\<^sub>r \<cdot> right_inject x"
+
+fun assemble_context\<^sub>c\<^sub>e :: "name \<Rightarrow> nat \<Rightarrow> (name \<times> type list) list \<Rightarrow> (name \<rightharpoonup> expr)" where
+  "assemble_context\<^sub>c\<^sub>e n depth [] = Map.empty"
+| "assemble_context\<^sub>c\<^sub>e n depth ((x, t) # cts) = 
+    (assemble_context\<^sub>c\<^sub>e n (Suc depth) cts)(x \<mapsto> \<succ>\<^bsub>n\<^esub> \<cdot> right_inject depth)"
+
+fun assemble_context\<^sub>c\<^sub>v :: "name \<Rightarrow> (name \<times> type list) list \<Rightarrow> (name \<rightharpoonup> val)" where
+  "assemble_context\<^sub>c\<^sub>v n [] = Map.empty"
+| "assemble_context\<^sub>c\<^sub>v n ((x, t) # cts) = (assemble_context\<^sub>c\<^sub>v n cts)(x \<mapsto> UnitV)" (* TODO! *)
+
+primrec assemble_context' :: "decl \<Rightarrow> dynamic_environment" where
+  "assemble_context' (TypeDecl x cts) = \<lparr> 
+    var\<^sub>e_bind = assemble_context\<^sub>c\<^sub>e x 0 cts, 
+    var\<^sub>v_bind = assemble_context\<^sub>c\<^sub>v x cts, 
+    var\<^sub>t_bind = [x \<mapsto> typecheck\<^sub>c\<^sub>t cts] \<rparr>"
+| "assemble_context' (ValDecl x v) = empty_dynamic \<lparr> var\<^sub>v_bind := [x \<mapsto> v] \<rparr>"
+| "assemble_context' (ExprDecl x e) = empty_dynamic \<lparr> var\<^sub>e_bind := [x \<mapsto> e] \<rparr>"
+
+primrec assemble_context :: "decl list \<Rightarrow> dynamic_environment" where
+  "assemble_context [] = empty_dynamic"
+| "assemble_context (\<delta> # \<Lambda>) = combine\<^sub>d (assemble_context' \<delta>) (assemble_context \<Lambda>)"
 
 primrec is_completed :: "prog \<Rightarrow> bool" where
   "is_completed (Prog \<Lambda> e v) = (e = \<epsilon>)"
 
 inductive evaluate_prog :: "prog \<Rightarrow> prog \<Rightarrow> bool" (infix "\<leadsto>" 60) where
-  ev_prog [simp]: "Map.empty & Map.empty \<Turnstile> \<Lambda> :: \<Gamma> & \<Sigma> \<Longrightarrow> 
-    assemble_context \<Lambda> & \<Sigma> \<turnstile> e \<cdot> v \<leadsto> e' \<cdot> v' \<Longrightarrow> Prog \<Lambda> e v \<leadsto> Prog \<Lambda> e' v'"
+  ev_prog [simp]: "assemble_context \<Lambda> \<turnstile> e \<cdot> v \<leadsto> e' \<cdot> v' \<Longrightarrow> Prog \<Lambda> e v \<leadsto> Prog \<Lambda> e' v'"
 
 inductive_cases [elim]: "Prog \<Lambda> e v \<leadsto> \<Pi>"
 
 (* safety *)
 
-lemma [simp]: "assemble_context (\<Lambda> @ \<Lambda>') = assemble_context \<Lambda> ++ assemble_context \<Lambda>'"
-  by (induction \<Lambda>) simp_all
+lemma [simp]: "combine\<^sub>d empty_dynamic \<Lambda> = \<Lambda>"
+  by (simp add: combine\<^sub>d_def empty_dynamic_def)
 
-lemma [simp]: "x \<notin> fst ` set cts \<Longrightarrow> x \<notin> dom (assemble_context\<^sub>c F cts)"
-  by (induction cts rule: assemble_context\<^sub>c.induct) simp_all
+lemma [simp]: "combine\<^sub>d \<Lambda> empty_dynamic = \<Lambda>"
+  by (simp add: combine\<^sub>d_def empty_dynamic_def)
 
-lemma [simp]: "x \<notin> binders\<^sub>d a \<Longrightarrow> x \<notin> dom (assemble_context' a)"
-  by (induction a) simp_all
+lemma [simp]: "combine\<^sub>d (combine\<^sub>d \<Lambda>\<^sub>1 \<Lambda>\<^sub>2) \<Lambda>\<^sub>3 = combine\<^sub>d \<Lambda>\<^sub>1 (combine\<^sub>d \<Lambda>\<^sub>2 \<Lambda>\<^sub>3)"
+  by (simp add: combine\<^sub>d_def empty_dynamic_def)
 
-lemma [simp]: "x \<notin> binders \<Lambda> \<Longrightarrow> x \<notin> dom (assemble_context \<Lambda>)"
-  by (induction \<Lambda>) simp_all
+lemma [simp]: "combine\<^sub>d \<Lambda> (empty_dynamic\<lparr>var\<^sub>e_bind := [x \<mapsto> e]\<rparr>) = extend\<^sub>e\<^sub>d x e \<Lambda>"
+  by (simp add: combine\<^sub>d_def empty_dynamic_def extend\<^sub>e\<^sub>d_def)
 
-lemma [simp]: "bind_with_names x Map.empty = Map.empty"
-  by auto
+lemma [simp]: "combine\<^sub>d \<Lambda> (empty_dynamic\<lparr>var\<^sub>v_bind := [x \<mapsto> v]\<rparr>) = extend\<^sub>v\<^sub>d x v \<Lambda>"
+  by (simp add: combine\<^sub>d_def empty_dynamic_def extend\<^sub>v\<^sub>d_def)
 
-lemma [simp]: "bind_with_names x (\<Gamma>(y \<mapsto> t)) = (bind_with_names x \<Gamma>)(y \<mapsto> (t, Named x))"
-  by auto
+lemma [simp]: "typecheck\<^sub>c\<^sub>e F cts x = Some (t\<^sub>1, t\<^sub>2) \<Longrightarrow> \<exists>e. assemble_context\<^sub>c\<^sub>e n d cts x = Some e"
+  by (induction F cts x arbitrary: d rule: typecheck\<^sub>c\<^sub>e.induct) auto
 
-lemma [simp]: "dom (assemble_context\<^sub>c x cts) = fst ` set cts"
-  proof (induction cts rule: assemble_context\<^sub>c.induct)
-  case (2 n x t cts)
-    hence "dom (assemble_context\<^sub>c n ((x, t) # cts)) = fst ` set ((x, t) # cts)" by simp
-    thus ?case by blast
+lemma [simp]: "assemble_context\<^sub>c\<^sub>e n d cts x = Some e \<Longrightarrow> \<exists>t\<^sub>1 t\<^sub>2. typecheck\<^sub>c\<^sub>e F cts x = Some (t\<^sub>1, t\<^sub>2)"
+  by (induction n d cts arbitrary: e rule: assemble_context\<^sub>c\<^sub>e.induct) auto
+
+lemma tc_assembled: "typecheck\<^sub>c\<^sub>e F cts x = Some (t\<^sub>1, t\<^sub>2) \<Longrightarrow> typecheck\<^sub>c\<^sub>t (cts' @ cts) = F \<Longrightarrow>
+  \<exists>e. assemble_context\<^sub>c\<^sub>e n (length cts') cts x = Some e \<and> \<lparr>var\<^sub>e_type = typecheck\<^sub>c\<^sub>e F cts, 
+    var\<^sub>v_type = typecheck\<^sub>c\<^sub>v F cts, var\<^sub>t_type = [n \<mapsto> F]\<rparr> \<turnstile> e : t\<^sub>1 \<rightarrow> t\<^sub>2"
+  proof (induction F cts x arbitrary: cts' rule: typecheck\<^sub>c\<^sub>e.induct)
+  case (2 F x ts cts y)
+    show ?case
+      proof (cases "x = y")
+      case True
+        with True 2 show ?thesis by simp
+      next case False
+        with False show ?thesis by simp
+      qed
   qed simp_all
 
-lemma add_constructors: "typecheck\<^sub>c cts = (\<Gamma>', F) \<Longrightarrow> \<Gamma> & \<Sigma> \<tturnstile> assemble_context \<Lambda> \<Longrightarrow> 
-  fst ` set cts \<inter> binders \<Lambda> = {} \<Longrightarrow> x \<notin> dom \<Sigma> \<Longrightarrow> distinct (map fst cts) \<Longrightarrow>
-    \<Gamma> ++ bind_with_names x \<Gamma>' & \<Sigma>(x \<mapsto> F) \<tturnstile> assemble_context \<Lambda> ++ assemble_context\<^sub>c x cts"
-  proof (induction cts arbitrary: \<Gamma>' F rule: typecheck\<^sub>c.induct)
-  case 1
-    hence "\<Gamma> & \<Sigma>(x \<mapsto> K \<zero>) \<tturnstile> assemble_context \<Lambda>" by simp
-    with 1 have "\<Gamma> ++ bind_with_names x \<Gamma>' & \<Sigma>(x \<mapsto> F) \<tturnstile> 
-      assemble_context \<Lambda> ++ assemble_context\<^sub>c x []" by fastforce
-    thus ?case by blast
-  next case (2 y ts cts)
-    then obtain \<Gamma>'' Fs where G: "typecheck\<^sub>c cts = (\<Gamma>'', Fs) \<and> \<Gamma>' = \<Gamma>''(y \<mapsto> foldr op \<otimes> ts \<one>) \<and> 
-      F = Fs \<Oplus> foldr (\<lambda>t. op \<Otimes> (K t)) ts (K \<one>)" by (auto split: prod.splits)
-    with 2 have "\<Gamma> ++ bind_with_names x \<Gamma>'' & \<Sigma>(x \<mapsto> Fs) \<tturnstile> 
-      assemble_context \<Lambda> ++ assemble_context\<^sub>c x cts" by fastforce
-
-
-    let ?t = "foldr op \<otimes> ts \<one>"
-    let ?F = "Fs \<Oplus> foldr (\<lambda>t. op \<Otimes> (K t)) ts (K \<one>)"
-    let ?\<Lambda> = "assemble_context \<Lambda> ++ (map_option (op \<cdot> \<iota>\<^sub>r) \<circ> assemble_context\<^sub>c x cts)"
-
-
-    from 2 have "\<Gamma> & \<Sigma> \<tturnstile> assemble_context \<Lambda>" by simp
-    from 2 have "y \<notin> binders \<Lambda>" by simp
-    from 2 have "fst ` set cts \<inter> binders \<Lambda> = {}" by simp
-    from 2 have "y \<notin> fst ` set cts" by simp
-    from 2 have "distinct (map fst cts)" by simp
-
-
-    have X: "(\<Gamma> ++ bind_with_names x \<Gamma>'') & \<Sigma>(x \<mapsto> ?F) \<turnstile> \<prec>\<^bsub>x\<^esub> \<cdot> \<iota>\<^sub>l : ?t \<rightarrow> Named x" by simp
-
-
-    have Y: "(\<Gamma> ++ bind_with_names x \<Gamma>'') & \<Sigma>(x \<mapsto> ?F) \<tturnstile> ?\<Lambda>" by simp
-
-
-    from 2 have "y \<notin> dom ?\<Lambda> " by simp
-    with X Y G have "\<Gamma> ++ bind_with_names x \<Gamma>' & \<Sigma>(x \<mapsto> F) \<tturnstile> 
-      assemble_context \<Lambda> ++ assemble_context\<^sub>c x ((y, ts) # cts)" by simp
-    thus ?case by blast
-  qed
-
-lemma assemble_postpend: "\<Gamma> & \<Sigma> \<Turnstile> \<delta> : \<Gamma>' & \<Sigma>' \<Longrightarrow> \<Gamma> & \<Sigma> \<tturnstile> assemble_context \<Lambda> \<Longrightarrow> 
-    binders\<^sub>d \<delta> \<inter> binders \<Lambda> = {} \<Longrightarrow> \<Gamma>' & \<Sigma>' \<tturnstile> assemble_context (\<Lambda> @ [\<delta>])"
-  proof (induction \<Gamma> \<Sigma> \<delta> \<Gamma>' \<Sigma>' rule: typecheck_decl.induct)
-  case (tcd_type cts \<Gamma>' F \<Gamma> \<Sigma> x)
-    hence "\<Gamma> ++ bind_with_names x \<Gamma>' & \<Sigma>(x \<mapsto> F) \<tturnstile> assemble_context (\<Lambda> @ [TypeDecl x cts])" 
-      using add_constructors by simp
-    thus ?case by blast
-  next case (tcd_expr \<Gamma> \<Sigma> e t\<^sub>1 t\<^sub>2 x)
-    hence "\<Gamma>(x \<mapsto> (t\<^sub>1, t\<^sub>2)) & \<Sigma> \<tturnstile> assemble_context (\<Lambda> @ [ExprDecl x e])" by simp
-    thus ?case by blast
-  qed
-
-lemma tc_assemble_context [simp]: "\<Gamma> & \<Sigma> \<Turnstile> \<Lambda>' :: \<Gamma>' & \<Sigma>' \<Longrightarrow> \<Gamma> & \<Sigma> \<tturnstile> assemble_context \<Lambda> \<Longrightarrow> 
-    binders \<Lambda> \<inter> binders \<Lambda>' = {} \<Longrightarrow> \<Gamma>' & \<Sigma>' \<tturnstile> assemble_context \<Lambda> ++ assemble_context \<Lambda>'"
-  proof (induction \<Gamma> \<Sigma> \<Lambda>' \<Gamma>' \<Sigma>' arbitrary: \<Lambda> rule: typecheck_decls.induct)
-  case tcd_nil
-    thus ?case by simp
-  next case (tcd_cons \<Gamma> \<Sigma> \<delta> \<Gamma>' \<Sigma>' \<Lambda>' \<Gamma>'' \<Sigma>'')
-    moreover hence "\<Gamma>' & \<Sigma>' \<tturnstile> assemble_context (\<Lambda> @ [\<delta>])" using assemble_postpend by fastforce
-    moreover from tcd_cons have "binders (\<Lambda> @ [\<delta>]) \<inter> binders \<Lambda>' = {}" by auto
-    ultimately have "\<Gamma>'' & \<Sigma>'' \<tturnstile> assemble_context (\<Lambda> @ [\<delta>]) ++ assemble_context \<Lambda>'" by blast
-    thus ?case by simp
-  qed
-
-lemma [simp]: "Map.empty & Map.empty \<Turnstile> \<Lambda> :: \<Gamma> & \<Sigma> \<Longrightarrow> \<Gamma> & \<Sigma> \<tturnstile> assemble_context \<Lambda>"
+lemma [simp]: "typecheck\<^sub>c\<^sub>e (typecheck\<^sub>c\<^sub>t cts) cts x = Some (t\<^sub>1, t\<^sub>2) \<Longrightarrow> 
+  \<exists>e. assemble_context\<^sub>c\<^sub>e n 0 cts x = Some e \<and> \<lparr>var\<^sub>e_type = typecheck\<^sub>c\<^sub>e (typecheck\<^sub>c\<^sub>t cts) cts, 
+    var\<^sub>v_type = typecheck\<^sub>c\<^sub>v (typecheck\<^sub>c\<^sub>t cts) cts, var\<^sub>t_type = [n \<mapsto> typecheck\<^sub>c\<^sub>t cts]\<rparr> \<turnstile> e : t\<^sub>1 \<rightarrow> t\<^sub>2"
   proof -
-    assume "Map.empty & Map.empty \<Turnstile> \<Lambda> :: \<Gamma> & \<Sigma>"
-    moreover have "Map.empty & Map.empty \<tturnstile> assemble_context []" by (simp add: typecheck_context_def)
-    ultimately show "\<Gamma> & \<Sigma> \<tturnstile> assemble_context \<Lambda>" using tc_assemble_context by fastforce
+    assume "typecheck\<^sub>c\<^sub>e (typecheck\<^sub>c\<^sub>t cts) cts x = Some (t\<^sub>1, t\<^sub>2)"
+    hence "typecheck\<^sub>c\<^sub>e (typecheck\<^sub>c\<^sub>t ([] @ cts)) cts x = Some (t\<^sub>1, t\<^sub>2)" by simp
+    thus ?thesis using tc_assembled by fastforce
+  qed
+
+lemma [simp]: "typecheck\<^sub>c\<^sub>v (typecheck\<^sub>c\<^sub>t cts) cts xa = Some t \<Longrightarrow> 
+  \<exists>v. assemble_context\<^sub>c\<^sub>v n cts xa = Some v \<and> \<lparr>var\<^sub>e_type = typecheck\<^sub>c\<^sub>e (typecheck\<^sub>c\<^sub>t cts) cts, 
+    var\<^sub>v_type = typecheck\<^sub>c\<^sub>v (typecheck\<^sub>c\<^sub>t cts) cts, var\<^sub>t_type = [n \<mapsto> typecheck\<^sub>c\<^sub>t cts]\<rparr> \<turnstile> v : t"
+  by simp
+
+lemma tc_typedecl: "typecheck\<^sub>d x cts \<tturnstile> assemble_context' (TypeDecl x cts)"
+  by (auto simp add: typecheck_environment_def typecheck\<^sub>d_def Let_def)
+
+lemma [simp]: "dom (typecheck\<^sub>c\<^sub>e x cts) = fst ` set cts"
+  by (induction cts rule: assemble_context\<^sub>c\<^sub>e.induct) (auto, force)
+
+lemma [simp]: "dom (typecheck\<^sub>c\<^sub>v x cts) = fst ` set cts"
+  by (auto simp add: typecheck\<^sub>c\<^sub>v_def) (force split: if_splits)+
+
+lemma [simp]: "domain\<^sub>s (typecheck\<^sub>d x cts) = insert x (fst ` set cts)"
+  by (simp add: domain\<^sub>s_def typecheck\<^sub>d_def Let_def)
+
+lemma [simp]: "\<Gamma>\<^sub>1 \<Turnstile> \<delta> : \<Gamma>\<^sub>2 \<Longrightarrow> \<Gamma>\<^sub>1 \<tturnstile> \<Lambda>\<^sub>1 \<Longrightarrow> binders\<^sub>d \<delta> \<inter> domain\<^sub>s \<Gamma>\<^sub>1 = {} \<Longrightarrow> 
+    \<Gamma>\<^sub>2 \<tturnstile> combine\<^sub>d \<Lambda>\<^sub>1 (assemble_context' \<delta>)"
+  proof (induction \<Gamma>\<^sub>1 \<delta> \<Gamma>\<^sub>2 rule: typecheck_decl.induct)
+  case (tcd_type \<Gamma> x cts)
+    hence "domain\<^sub>s \<Gamma> \<inter> domain\<^sub>s (typecheck\<^sub>d x cts) = {}" by auto
+    with tcd_type show ?case by (metis typecheck_combine tc_typedecl)
+  qed simp_all
+
+lemma tc_defs_parts [simp]: "\<Gamma>\<^sub>1 \<Turnstile> \<Lambda>\<^sub>2 :: \<Gamma>\<^sub>2 \<Longrightarrow> \<Gamma>\<^sub>1 \<tturnstile> \<Lambda>\<^sub>1 \<Longrightarrow> \<Gamma>\<^sub>2 \<tturnstile> combine\<^sub>d \<Lambda>\<^sub>1 (assemble_context \<Lambda>\<^sub>2)"
+  proof (induction \<Gamma>\<^sub>1 \<Lambda>\<^sub>2 \<Gamma>\<^sub>2 arbitrary: \<Lambda>\<^sub>1 rule: typecheck_decls.induct)
+  case (tcd_cons \<Gamma>\<^sub>1 \<delta> \<Gamma>\<^sub>2 \<Lambda>\<^sub>2 \<Gamma>\<^sub>3)
+    moreover hence "\<Gamma>\<^sub>2 \<tturnstile> combine\<^sub>d \<Lambda>\<^sub>1 (assemble_context' \<delta>)" by simp
+    ultimately show ?case by fastforce
+  qed simp_all
+
+lemma [simp]: "empty_static \<tturnstile> empty_dynamic" 
+  by (simp add: typecheck_environment_def empty_static_def empty_dynamic_def)
+
+lemma [simp]: "empty_static \<Turnstile> \<Lambda> :: \<Gamma> \<Longrightarrow> \<Gamma> \<tturnstile> assemble_context \<Lambda>"
+  proof -
+    assume "empty_static \<Turnstile> \<Lambda> :: \<Gamma>"
+    moreover have "empty_static \<tturnstile> empty_dynamic" by simp
+    ultimately have "\<Gamma> \<tturnstile> combine\<^sub>d empty_dynamic (assemble_context \<Lambda>)" by (metis tc_defs_parts)
+    thus "\<Gamma> \<tturnstile> assemble_context \<Lambda>" by simp
   qed                                                                  
 
-theorem progress [simp]: "\<Pi> \<TTurnstile> \<Gamma> & \<Sigma> : t \<Longrightarrow> is_completed \<Pi> \<or> (\<exists>\<Pi>'. \<Pi> \<leadsto> \<Pi>')"
-  proof (induction \<Pi> \<Gamma> \<Sigma> t rule: typecheck_prog.induct)
-  case (tcp_prog \<Lambda> \<Gamma> \<Sigma> e t\<^sub>1 t\<^sub>2 v)
+theorem progress [simp]: "\<Pi> \<TTurnstile> \<Gamma> \<rightarrow> t \<Longrightarrow> is_completed \<Pi> \<or> (\<exists>\<Pi>'. \<Pi> \<leadsto> \<Pi>')"
+  proof (induction \<Pi> \<Gamma> t rule: typecheck_prog.induct)
+  case (tcp_prog \<Lambda> \<Gamma> e t\<^sub>1 t\<^sub>2 v)
     thus ?case 
       proof (cases "e = \<epsilon>")
       case False
-        with tcp_prog obtain e' v' where "assemble_context \<Lambda> & \<Sigma> \<turnstile> e \<cdot> v \<leadsto> e' \<cdot> v'" by fastforce
+        with tcp_prog obtain e' v' where "assemble_context \<Lambda> \<turnstile> e \<cdot> v \<leadsto> e' \<cdot> v'" by fastforce
         with tcp_prog have "Prog \<Lambda> e v \<leadsto> Prog \<Lambda> e' v'" by simp
         thus ?thesis by fastforce
       qed simp_all
   qed
 
-lemma [simp]: "\<Gamma> & \<Sigma> \<Turnstile> \<delta> : \<Gamma>\<^sub>1 & \<Sigma>\<^sub>1 \<Longrightarrow> \<Gamma> & \<Sigma> \<Turnstile> \<delta> : \<Gamma>\<^sub>1' & \<Sigma>\<^sub>1' \<Longrightarrow> \<Gamma>\<^sub>1 = \<Gamma>\<^sub>1' \<and> \<Sigma>\<^sub>1 = \<Sigma>\<^sub>1'"
-  proof (induction \<Gamma> \<Sigma> \<delta> \<Gamma>\<^sub>1 \<Sigma>\<^sub>1 rule: typecheck_decl.induct)
-  case (tcd_expr \<Gamma> \<Sigma> e t\<^sub>1 t\<^sub>2 x)
-    thus ?case by simp
-  qed auto
-
-lemma [simp]: "\<Gamma> & \<Sigma> \<Turnstile> \<Lambda> :: \<Gamma>\<^sub>1 & \<Sigma>\<^sub>1 \<Longrightarrow> \<Gamma> & \<Sigma> \<Turnstile> \<Lambda> :: \<Gamma>\<^sub>1' & \<Sigma>\<^sub>1' \<Longrightarrow> \<Gamma>\<^sub>1 = \<Gamma>\<^sub>1' \<and> \<Sigma>\<^sub>1 = \<Sigma>\<^sub>1'"
-  proof (induction \<Gamma> \<Sigma> \<Lambda> \<Gamma>\<^sub>1 \<Sigma>\<^sub>1 rule: typecheck_decls.induct)
-  case (tcd_cons \<Gamma> \<Sigma> \<delta> \<Gamma>\<^sub>2 \<Sigma>\<^sub>2 \<Lambda> \<Gamma>\<^sub>1 \<Sigma>\<^sub>1)
-    moreover then obtain \<Gamma>\<^sub>2' \<Sigma>\<^sub>2' where "(\<Gamma> & \<Sigma> \<Turnstile> \<delta> : \<Gamma>\<^sub>2' & \<Sigma>\<^sub>2') \<and> \<Gamma>\<^sub>2' & \<Sigma>\<^sub>2' \<Turnstile> \<Lambda> :: \<Gamma>\<^sub>1' & \<Sigma>\<^sub>1'" 
-      by fastforce
-    moreover with tcd_cons have "\<Gamma>\<^sub>2 = \<Gamma>\<^sub>2' \<and> \<Sigma>\<^sub>2 = \<Sigma>\<^sub>2'" by fastforce
-    ultimately show ?case by simp
-  qed auto
-
-theorem preservation [simp]: "\<Pi> \<leadsto> \<Pi>' \<Longrightarrow> \<Pi> \<TTurnstile> \<Gamma> & \<Sigma> : t \<Longrightarrow> \<Pi>' \<TTurnstile> \<Gamma> & \<Sigma> : t"
+theorem preservation [simp]: "\<Pi> \<leadsto> \<Pi>' \<Longrightarrow> \<Pi> \<TTurnstile> \<Gamma> \<rightarrow> t \<Longrightarrow> \<Pi>' \<TTurnstile> \<Gamma> \<rightarrow> t"
   proof (induction \<Pi> \<Pi>' rule: evaluate_prog.induct)
-  case (ev_prog \<Lambda> \<Gamma>' \<Sigma>' e v e' v')
-    moreover then obtain t\<^sub>1 where T: "(Map.empty & Map.empty \<Turnstile> \<Lambda> :: \<Gamma> & \<Sigma>) \<and> 
-      (\<Gamma> & \<Sigma> \<turnstile> e : t\<^sub>1 \<rightarrow> t) \<and> \<Gamma> & \<Sigma> \<turnstile> v : t\<^sub>1" by blast
-    moreover with ev_prog have "\<Gamma> = \<Gamma>' \<and> \<Sigma> = \<Sigma>'" by fastforce
-    ultimately obtain t\<^sub>2 where "(\<Gamma> & \<Sigma> \<turnstile> e' : t\<^sub>2 \<rightarrow> t) \<and> (\<Gamma> & \<Sigma> \<turnstile> v' : t\<^sub>2)" by fastforce
+  case (ev_prog \<Lambda> e v e' v')
+    moreover then obtain t\<^sub>1 where T: "(empty_static \<Turnstile> \<Lambda> :: \<Gamma>) \<and> (\<Gamma> \<turnstile> e : t\<^sub>1 \<rightarrow> t) \<and> \<Gamma> \<turnstile> v : t\<^sub>1" 
+      by blast
+    ultimately obtain t\<^sub>2 where "(\<Gamma> \<turnstile> e' : t\<^sub>2 \<rightarrow> t) \<and> (\<Gamma> \<turnstile> v' : t\<^sub>2)" by fastforce
     with T show ?case by fastforce
   qed
 
@@ -219,28 +214,21 @@ inductive total_evaluate_prog :: "prog \<Rightarrow> val \<Rightarrow> bool" (in
 | ptev_step [simp]: "Prog \<Lambda> e v \<leadsto> Prog \<Lambda> e' v' \<Longrightarrow> Prog \<Lambda> e' v' \<Down> v'' \<Longrightarrow> Prog \<Lambda> e v \<Down> v''"
 
 inductive total_evaluate_prog' :: "prog \<Rightarrow> val \<Rightarrow> bool" (infix "\<Down>\<Down>" 60) where
-  ptev_step' [simp]: "Map.empty & Map.empty \<Turnstile> \<Lambda> :: \<Gamma> & \<Sigma> \<Longrightarrow> 
-    assemble_context \<Lambda> & \<Sigma> \<turnstile> e \<cdot> v \<Down> v' \<Longrightarrow> Prog \<Lambda> e v \<Down>\<Down> v'"
+  ptev_step' [simp]: "assemble_context \<Lambda> \<turnstile> e \<cdot> v \<Down> v' \<Longrightarrow> Prog \<Lambda> e v \<Down>\<Down> v'"
 
 inductive_cases [elim]: "Prog \<Lambda> e v \<Down>\<Down> v'"
 
 lemma [simp]: "\<Pi> \<Down> v = \<Pi> \<Down>\<Down> v"
   proof
-    show "\<Pi> \<Down> v \<Longrightarrow> \<Pi> \<Down>\<Down> v" 
-      proof (induction \<Pi> v rule: total_evaluate_prog.induct) 
-      case ptev_base
-        thus ?case by simp
-      next case ptev_step
-        thus ?case by simp
-      qed
+    show "\<Pi> \<Down> v \<Longrightarrow> \<Pi> \<Down>\<Down> v" by (induction \<Pi> v rule: total_evaluate_prog.induct) fastforce+
   next 
     assume "\<Pi> \<Down>\<Down> v"
     thus "\<Pi> \<Down> v"
       proof (induction \<Pi> v rule: total_evaluate_prog'.induct)
-      case (ptev_step' \<Lambda> \<Gamma> \<Sigma> e v v')
-        with ptev_step'(2) show ?case 
-          proof (induction "assemble_context \<Lambda>" \<Sigma> e v v' rule: total_eval.induct)
-          case (tev_step \<Sigma> e v e' v' v'')
+      case (ptev_step' \<Lambda> e v v')
+        thus ?case 
+          proof (induction "assemble_context \<Lambda>" e v v' rule: total_eval.induct)
+          case (tev_step e v e' v' v'')
             moreover hence "Prog \<Lambda> e v \<leadsto> Prog \<Lambda> e' v'" by simp
             ultimately show ?case by (metis total_evaluate_prog.ptev_step)
           qed simp_all
@@ -249,10 +237,10 @@ lemma [simp]: "\<Pi> \<Down> v = \<Pi> \<Down>\<Down> v"
 
 (* since we are a turing-complete language, total progress is not provable *)
 
-lemma [simp]: "\<Pi> \<Down>\<Down> v \<Longrightarrow> \<Pi> \<TTurnstile> \<Gamma> & \<Sigma> : t \<Longrightarrow> \<Gamma> & \<Sigma> \<turnstile> v : t"
+lemma [simp]: "\<Pi> \<Down>\<Down> v \<Longrightarrow> \<Pi> \<TTurnstile> \<Gamma> \<rightarrow> t \<Longrightarrow> \<Gamma> \<turnstile> v : t"
   by (induction \<Pi> v rule: total_evaluate_prog'.induct) auto
 
-theorem total_preservation: "\<Pi> \<Down> v \<Longrightarrow> \<Pi> \<TTurnstile> \<Gamma> & \<Sigma> : t \<Longrightarrow> \<Gamma> & \<Sigma> \<turnstile> v : t"
+theorem total_preservation: "\<Pi> \<Down> v \<Longrightarrow> \<Pi> \<TTurnstile> \<Gamma> \<rightarrow> t \<Longrightarrow> \<Gamma> \<turnstile> v : t"
   by simp
 
 end
